---
layout: post
title:  $\int log(\sqrt{x} + \sqrt{x + 1})dx$
date:   2021-01-31 10:08:15 - 0700
categories: integrals
---

<script type="text/x-mathjax-config">
MathJax.Hub.Config({
  tex2jax: {
    inlineMath: [['$','$'], ['\\(','\\)']],
    processEscapes: true
  }
});
</script>

<script src="https://cdnjs.cloudflare.com/ajax/libs/mathjax/2.7.0/MathJax.js?config=TeX-AMS-MML_HTMLorMML" type="text/javascript"></script>

Assume $x\in\mathbf{R}$ and that $x > 0$. We could have $x = 0$, but the solution has a removable pole at x = 0, see the solution for an explanation.

$$ = xlog(\sqrt{x} + \sqrt{x + 1}) - \int \frac{x}{\sqrt{x} + \sqrt{x + 1}}(\frac{1}{2\sqrt{x}} + \frac{1}{2\sqrt{x + 1}})dx $$

$$ = xlog(\sqrt{x} + \sqrt{x + 1}) - \frac{1}{2}\int \frac{x}{\sqrt{x^2 + x}} dx $$

$$ = xlog(\sqrt{x} + \sqrt{x + 1}) - \frac{1}{2}\int (\frac{x}{\sqrt{x}})(\frac{1}{\sqrt{x + 1}}) dx $$

$$ = xlog(\sqrt{x} + \sqrt{x + 1}) - \frac{1}{2}(2\sqrt{x + 1}\frac{x}{\sqrt{x}} - \int 2\sqrt{x + 1}(\frac{\sqrt{x} - \frac{x}{2\sqrt{x}}}{x})dx) $$

$$ = xlog(\sqrt{x} + \sqrt{x + 1}) - \frac{1}{2}(2\frac{x\sqrt{x + 1}}{\sqrt{x}} - \int \frac{\sqrt{x + 1}}{\sqrt{x}} dx) $$

$$ u = \sqrt{x} $$

$$ = xlog(\sqrt{x} + \sqrt{x + 1}) - \frac{1}{2}(2\frac{x\sqrt{x + 1}}{\sqrt{x}} - 2\int \frac{\sqrt{u^2 + 1}}{u}u du) $$

$$ = xlog(\sqrt{x} + \sqrt{x + 1}) - \frac{1}{2}(2\frac{x\sqrt{x + 1}}{\sqrt{x}} - 2\int \sqrt{u^2 + 1}du) $$


***
#### A Necessary Integral

Note The Following Integral:

$$ I = \int \sqrt{u^2 + 1} du = u\sqrt{u^2 + 1} - \int \frac{u^2}{\sqrt{u^2 + t}} du $$

$$ = u\sqrt{u^2 + 1} - \int \frac{u^2 + 1}{\sqrt{u^2 + t}} - \frac{1}{\sqrt{u^2 + 1}} du $$

$$ u\sqrt{u^2 + 1} - \int \sqrt{u^2 + t} du - \int \frac{1}{\sqrt{u^2 + 1}} du$$

$$ = u\sqrt{u^2 + 1} - I - arcsinh(u)$$

$$ I = \frac{1}{2}(u\sqrt{u^2 + 1} - arcsinh(u)) $$

$$ = \frac{1}{2}(\sqrt{x}\sqrt{x + 1} - arcsinh(\sqrt{x})) $$

***
#### Putting Everything Together

$$ = xlog(\sqrt{x} + \sqrt{x + 1}) - \frac{1}{2}(2  \frac{x\sqrt{x + 1}}{\sqrt{x}}  - 2(\frac{1}{2}(\sqrt{x}\sqrt{x + 1} - arcsinh(\sqrt{x})))) $$

$$ = xlog(\sqrt{x} + \sqrt{x + 1}) - \frac{x\sqrt{x + 1}}{\sqrt{x}} + \frac{1}{2}\sqrt{x^2 + x} - \frac{1}{2}arcsinh(\sqrt{x}) $$

$$ = xlog(\sqrt{x} + \sqrt{x + 1}) - \frac{1}{2}\sqrt{x^2 + x} - \frac{1}{2}arcsinh(\sqrt{x}) $$

$$ = \boxed{(x - \frac{1}{2})log(\sqrt{x} + \sqrt{x + 1}) - \frac{1}{2}\sqrt{x^2 + x} + C} $$

***
#### arcsinh Expressed Algebraically

The last step used the following identity for $arcsinh$:

$$ z = sinh(x) = \frac{e^x - e^{-x}}{2} $$

$$ = \frac{e^x - e^{-x}}{2}\frac{e^x}{e^x} $$

$$ = \frac{e^{2x} - 1}{2e^x} $$

$$ 2ze^x = e^{2x} - 1 $$

$$ (e^{x})^2 - 2z(e^x) - 1 = 0 $$

$$ e^x = \frac{2z + \sqrt{4z^2 + 4}}{2} $$

$$ = z + \sqrt{z^2 + 1} $$

$$ x = arcsinh(z) = log(z + \sqrt{z^2 + 1}) $$

$$ arcsinh(\sqrt{x}) = \boxed{log(\sqrt{x} + \sqrt{x + 1})} $$

***
#### Poles and Analytic Continuation

The second to last step removed the removable singularity $x = 0$. So we define the new function on the analytic continuation of $\frac{x}{\sqrt{x}}$ taking value $0$ at $x = 0$, and the function is now well defined at $x = 0$. 
